new features + weakly closed subj. red
- added e_det in expr
- proved transitivity of subtype
- closed subject reduction up to 3.19, and more sublemmas related to wfc and existence of projections

process/beta.v
@@ -1,78 +1,318 @@
-From SST Require Export src.unscoped src.expressions process.processes process.sessions.
+From SST Require Export src.unscoped src.expressions process.processes process.sessions process.substitution.
 Require Import List String Relations ZArith.
 Require Import Setoid Morphisms Coq.Program.Basics.
 Import ListNotations.
 Require Import Coq.Init.Datatypes.
 
-Inductive multi {X : Type} (R : relation X) : relation X :=
-  | multi_refl : forall (x : X), multi R x x 
-  | multi_step : forall (x y z : X), R x y -> multi R y z -> multi R x z.
-  
-Lemma transitive_multi {X : Type} : forall (R : relation X) (x y z : X), multi R x y -> multi R y z -> multi R x z.
-Proof.
-  intros R x y z H.
-  revert z.
-  induction H; intros. easy.
-  specialize(IHmulti z0 H1).
-  specialize(@multi_step X R); intros.
-  apply H2 with (y := y). easy. easy.
-Qed.
 
-
-(* substitute e into e_var n of e1 *)
-Fixpoint subst_expr (n : fin) (e : expr) (e1 : expr) : expr :=
+(* substitute e into e_var n of e1, depth d *)
+Fixpoint subst_expr (n d : fin) (e : expr) (e1 : expr) : expr :=
   match e1 with 
-    | e_var 0     => if Nat.eqb n 0 then e else e_var 0
-    | e_var (S m) => if Nat.eqb (S m) n then e else 
+    | e_var 0     => if Nat.eqb n 0 then (incr_freeE 0 d e) else e_var 0
+    | e_var (S m) => if Nat.eqb (S m) n then (incr_freeE 0 d e) else 
                      if Nat.ltb (S m) n then e_var (S m) else e_var m 
-    | e_succ e' => e_succ (subst_expr n e e')
-    | e_neg e' => e_neg (subst_expr n e e')
-    | e_not e' => e_not (subst_expr n e e')
-    | e_gt e' e'' => e_gt (subst_expr n e e') (subst_expr n e e'')
-    | e_plus e' e'' => e_plus (subst_expr n e e') (subst_expr n e e'')
+    | e_succ e' => e_succ (subst_expr n d e e')
+    | e_neg e' => e_neg (subst_expr n d e e')
+    | e_not e' => e_not (subst_expr n d e e')
+    | e_gt e' e'' => e_gt (subst_expr n d e e') (subst_expr n d e e'')
+    | e_plus e' e'' => e_plus (subst_expr n d e e') (subst_expr n d e e'')
+    | e_det e' e'' => e_det (subst_expr n d e e') (subst_expr n d e e'')
     | _ => e1
   end.
   
-(* For a choice function, substitutes expr to e_var 0 (decr everything else), return process continuation of choice with label l with e substituted for e_var 0. anything else is kept as is. If label doesn't appear in the list we return p
+(* For a choice function, substitutes expr to e_var n (decr vars above n), d keeps track of depth of recv return process continuation
  *)
  
-
-Definition subst_expr_proc (p : process) (lb : label) (e : expr) : (option process) :=
-  match p with
-    | p_recv pt lst => 
-      match nth lb lst None with 
-        | None => None 
-        | Some y => let fix rec n p' := 
-          match p' with 
-            | p_send pt' l' e' P' => p_send pt' l' (subst_expr n e e') (rec (S n) P')
-            | p_ite e' P' Q'      => p_ite (subst_expr n e e') (rec n P') (rec n Q')
-            | p_recv pt' lst'     => p_recv pt' (list_map (fun x => match x with 
-                                                          | None => None
-                                                          | Some y => Some (rec n y) end) lst')
-            | p_rec P' => p_rec (rec n P')
-            | _ => p'
-          end 
-          in Some (rec 0 y)
-      end 
-    | _ => None 
+Fixpoint subst_expr_proc (p : process) (e : expr) (n d : fin) : process :=
+  match p with 
+    | p_send pt l e' P => p_send pt l (subst_expr n d e e') (subst_expr_proc P e n d)
+    | p_ite e' P Q     => p_ite (subst_expr n d e e') (subst_expr_proc P e n d) (subst_expr_proc Q e n d)
+    | p_recv pt lst    => p_recv pt (list_map (fun x => match x with
+                                                | None => None
+                                                | Some y => Some (subst_expr_proc y e (S n) (S d))
+                                               end) lst)
+    | p_rec P          => p_rec (subst_expr_proc P e n d)
+    | _ => p
   end.
 
+
 Inductive betaP: relation session :=
-  | r_comm  : forall p q xs l e Q M,
+  | r_comm  : forall p q xs y l e v Q M, 
+              onth l xs = Some y -> stepE_multi e v -> 
               betaP ((p <-- (p_recv q xs)) ||| (q <-- (p_send p l e Q)) ||| M)
-                    ((p <-- subst_expr_proc (p_recv q xs) l e) ||| (q <-- Q) ||| M)
-  | rt_ite  : forall p P Q M,
-              betaP ((p <-- (p_ite (e_val (vbool true)) P Q)) ||| M) ((p <-- P) ||| M)
-  | rf_ite  : forall p P Q M,
-              betaP ((p <-- (p_ite (e_val (vbool false)) P Q)) ||| M) ((p <-- Q) ||| M)
+                    ((p <-- subst_expr_proc y v 0 0) ||| (q <-- Q) ||| M)
+  | rt_ite  : forall p e P Q M,
+              stepE_multi e (e_val (vbool true)) ->
+              betaP ((p <-- (p_ite e P Q)) ||| M) ((p <-- P) ||| M)
+  | rf_ite  : forall p e P Q M,
+              stepE_multi e (e_val (vbool false)) ->
+              betaP ((p <-- (p_ite e P Q)) ||| M) ((p <-- Q) ||| M)
   | r_struct: forall M1 M1' M2 M2', scong M1 M1' -> scong M2' M2 -> betaP M1' M2' -> betaP M1 M2.
 
 Definition beta_multistep := multi betaP.
 
+Lemma onth_sless {X} : forall n (Gsl Gsr : list (option X)) x0 S,
+      n < length Gsl ->
+      onth n (Gsl ++ Some S :: Gsr) = Some x0 ->
+      onth n (Gsl ++ Gsr) = Some x0.
+Proof.
+  intro n. induction n; intros; try easy.
+  - destruct Gsl; try easy.
+  - destruct Gsl; try easy. apply IHn with (S := S); try easy.
+  apply PeanoNat.lt_S_n; try easy.
+Qed.
+
+Lemma onth_smore {X} : forall n (Gsl Gsr : list (option X)) x0 o S,
+      n <> length Gsl ->
+      length Gsl <= n ->
+      Some x0 = onth n (Gsl ++ Some S :: Gsr) ->
+      Some x0 = onth n (o :: Gsl ++ Gsr).
+Proof.
+  intro n. induction n; intros; try easy.
+  destruct Gsl; try easy.
+  simpl in *. destruct Gsl; try easy.
+  apply IHn with (S := S); try easy. simpl in *.
+  specialize(Nat.succ_inj_wd_neg n (length Gsl)); intros. destruct H2. specialize(H2 H). easy.
+  apply le_S_n; try easy.
+Qed.
+
+Lemma expr_subst : forall v ex x d Gsl Gsr S,
+        typ_expr (Gsl ++ Gsr) (incr_freeE 0 d v) S ->
+        typ_expr (Gsl ++ Some S :: Gsr) ex x ->
+        typ_expr (Gsl ++ Gsr) (subst_expr (length Gsl) d v ex) x.
+Proof.
+  intros v ex. revert v.
+  induction ex; intros; try easy.
+  - simpl in *.
+    specialize(inv_expr_var (e_var n) n (Gsl ++ Some S :: Gsr) x H0 (eq_refl (e_var n))); intros.
+    destruct H1. destruct H1. 
+    apply sc_sub with (s := x0); try easy.
+    - destruct n; try easy.
+      case_eq (Nat.eqb (length Gsl) 0); intros; try easy.
+      destruct Gsl; try easy. simpl in *. inversion H1. subst. easy.
+    - destruct Gsl; try easy. constructor; try easy.
+    destruct Gsl.
+    - simpl in *. constructor; try easy.
+    - simpl in *.
+      case_eq (Nat.eqb n (length Gsl)); intros.
+      - specialize(onth_exact Gsl Gsr (Some S)); intros.
+        specialize(natb_to_prop n (length Gsl) H3); intros. subst.
+        specialize(eq_trans (eq_sym H1) H4); intros. inversion H5. subst. easy.
+      case_eq (Datatypes.S n <? Datatypes.S (length Gsl))%nat; intros.
+      - specialize(Nat.ltb_lt (Datatypes.S n) (Datatypes.S (length Gsl))); intros.
+        destruct H5. specialize(H5 H4). clear H4 H6.
+        constructor.
+        apply eq_sym. apply onth_sless with (S := S); try easy.
+        apply PeanoNat.lt_S_n. easy.
+      - specialize(Nat.ltb_ge(Datatypes.S n) (Datatypes.S (length Gsl))); intros.
+        destruct H5. specialize(H5 H4). clear H4 H6.
+        constructor.
+        apply onth_smore with (S := S); try easy.
+        apply natb_to_propf. easy.
+        apply le_S_n. easy.
+  - simpl in *.
+    specialize(inv_expr_vali (Gsl ++ Some S :: Gsr) (e_val v) x v H0 (eq_refl (e_val v))); intros.
+    destruct H1.
+    - destruct H1. destruct H1. subst. apply sc_vali.
+    - destruct H1. destruct H1. destruct H1. subst. apply sc_sub with (s := snat); try easy. apply sc_valn.
+    - destruct H1. destruct H1. subst. apply sc_valb.
+  - simpl in *.
+    specialize(inv_expr_succ (Gsl ++ Some S :: Gsr) (e_succ ex) x ex H0 (eq_refl (e_succ ex))); intros.
+    destruct H1. destruct H2.
+    - subst. apply sc_succ. apply IHex with (S := S); try easy.
+    - subst. apply sc_sub with (s := snat); try easy. apply sc_succ. apply IHex with (S := S); try easy.
+      apply sni.
+  - simpl in *.
+    specialize(inv_expr_neg (Gsl ++ Some S :: Gsr) (e_neg ex) x ex H0 (eq_refl (e_neg ex))); intros.
+    destruct H1. subst. constructor. apply IHex with (S := S); try easy.
+  - simpl in *.
+    specialize(inv_expr_not (Gsl ++ Some S :: Gsr) (e_not ex) x ex H0 (eq_refl (e_not ex))); intros.
+    destruct H1. subst. constructor. apply IHex with (S := S); try easy.
+  - simpl in *.
+    specialize(inv_expr_gt (Gsl ++ Some S :: Gsr) (e_gt ex1 ex2) x ex1 ex2 H0 (eq_refl (e_gt ex1 ex2))); intros.
+    destruct H1. destruct H2. subst.
+    constructor. apply IHex1 with (S := S); try easy. apply IHex2 with (S := S); try easy.
+  - simpl in *.
+    specialize(inv_expr_plus (Gsl ++ Some S :: Gsr) (e_plus ex1 ex2) x ex1 ex2 H0 (eq_refl (e_plus ex1 ex2))); intros.
+    destruct H1. destruct H2. subst.
+    constructor. apply IHex1 with (S := S); try easy. apply IHex2 with (S := S); try easy.
+  - simpl in *.
+    specialize(inv_expr_det (Gsl ++ Some S :: Gsr) (e_det ex1 ex2) x ex1 ex2 H0 (eq_refl (e_det ex1 ex2))); intros.
+    destruct H1. destruct H1. destruct H2.
+    apply sc_sub with (s := x0); try easy.
+    constructor. apply IHex1 with (S := S); try easy. apply IHex2 with (S := S); try easy.
+Qed.
+
+Lemma SList_map_a24 {A} : forall (llp : list (option process)) v d (Gsl : list A),
+  SList llp ->
+  SList
+  (list_map
+     (fun x0 : option process =>
+      match x0 with
+      | Some y =>
+          Some
+            (subst_expr_proc y v (Datatypes.S (length Gsl)) (Datatypes.S d))
+      | None => None
+      end) llp).
+Proof.
+  intro llp. induction llp; intros; try easy.
+  specialize(SList_induc a llp H); intros. destruct H0; subst; try easy. destruct a; try easy. 
+  apply SList_inducb. apply IHllp; try easy.
+Qed.
+
+Lemma slideE : forall v Gs d S x0,
+               typ_expr Gs (incr_freeE 0 d v) S ->
+               typ_expr (Some x0 ::Gs) (incr_freeE 0 (Datatypes.S d) v) S.
+Proof.
+  intro v. induction v; intros; try easy.
+  - simpl in H.
+    specialize(inv_expr_var (e_var (n + d)) (n + d) Gs S H (eq_refl (e_var (n + d)))); intros.
+    destruct H0. destruct H0. apply sc_sub with (s := x); try easy.
+    constructor. simpl.
+    specialize(Nat.add_succ_r n d); intros.
+    replace (n + Datatypes.S d) with (Datatypes.S (n + d)). simpl. easy.
+  - simpl in *.
+    specialize(inv_expr_vali Gs (e_val v) S v H (eq_refl (e_val v))); intros.
+    - destruct H0. destruct H0. destruct H0. subst. apply sc_vali.
+    - destruct H0. destruct H0. destruct H0. subst. apply sc_sub with (s := snat); try easy. apply sc_valn.
+    - destruct H0. destruct H0. subst. apply sc_valb.
+  - simpl in *.
+    specialize(inv_expr_succ Gs (e_succ (incr_freeE 0 d v)) S (incr_freeE 0 d v) H (eq_refl (e_succ (incr_freeE 0 d v)))); intros.
+    destruct H0. destruct H1. subst. constructor. apply IHv; try easy.
+    subst. apply sc_sub with (s := snat). constructor. apply IHv; try easy. apply sni.
+  - simpl in *.
+    specialize(inv_expr_neg Gs (e_neg (incr_freeE 0 d v)) S (incr_freeE 0 d v) H (eq_refl (e_neg (incr_freeE 0 d v)))); intros.
+    destruct H0. subst. constructor. apply IHv; try easy.
+  - simpl in *.
+    specialize(inv_expr_not Gs (e_not (incr_freeE 0 d v)) S (incr_freeE 0 d v) H (eq_refl (e_not (incr_freeE 0 d v)))); intros.
+    destruct H0. subst. constructor. apply IHv; try easy.
+  - simpl in *.
+    specialize(inv_expr_gt Gs (e_gt (incr_freeE 0 d v1) (incr_freeE 0 d v2)) S (incr_freeE 0 d v1) (incr_freeE 0 d v2) H (eq_refl (e_gt (incr_freeE 0 d v1) (incr_freeE 0 d v2)))); intros.
+    destruct H0. subst. constructor. apply IHv1; try easy. apply IHv2; try easy.
+  - simpl in *.
+    specialize(inv_expr_plus Gs (e_plus (incr_freeE 0 d v1) (incr_freeE 0 d v2)) S (incr_freeE 0 d v1) (incr_freeE 0 d v2) H (eq_refl (e_plus (incr_freeE 0 d v1) (incr_freeE 0 d v2)))); intros.
+    destruct H0. subst. constructor. apply IHv1; try easy. apply IHv2; try easy.
+  - simpl in *.
+    specialize(inv_expr_det Gs (e_det (incr_freeE 0 d v1) (incr_freeE 0 d v2)) S (incr_freeE 0 d v1) (incr_freeE 0 d v2) H (eq_refl (e_det (incr_freeE 0 d v1) (incr_freeE 0 d v2)))); intros.
+    destruct H0. destruct H0. destruct H1.
+    apply sc_sub with (s := x); try easy. constructor. apply IHv1; try easy. apply IHv2; try easy.
+Qed.
+
+
+Lemma _a24_helper_recv : forall llp Gsl Gsr Gt d v x S,
+    typ_expr (Gsl ++ Gsr) (incr_freeE 0 d v) S ->
+    Forall
+      (fun u : option process =>
+       match u with
+       | Some k =>
+           forall (v : expr) (d : fin) (Gsl Gsr : list (option sort)) (Gt : ctxT) (S : sort) (T : ltt),
+           typ_proc (Gsl ++ Some S :: Gsr) Gt k T ->
+           typ_expr (Gsl ++ Gsr) (incr_freeE 0 d v) S ->
+           typ_proc (Gsl ++ Gsr) Gt (subst_expr_proc k v (length Gsl) d) T
+       | None => True
+       end) llp ->
+    Forall2
+       (fun (u : option process) (v : option (sort * ltt)) =>
+        u = None /\ v = None \/
+        (exists (p : process) (s : sort) (t : ltt),
+           u = Some p /\ v = Some (s, t) /\ typ_proc (Some s :: Gsl ++ Some S :: Gsr) Gt p t)) llp x ->
+    Forall2
+        (fun (u : option process) (v0 : option (sort * ltt)) =>
+         u = None /\ v0 = None \/
+         (exists (p : process) (s : sort) (t : ltt),
+            u = Some p /\ v0 = Some (s, t) /\ typ_proc (Some s :: Gsl ++ Gsr) Gt p t))
+        (list_map
+           (fun x0 : option process =>
+            match x0 with
+            | Some y =>
+                Some
+                  (subst_expr_proc y v (Datatypes.S (length Gsl)) (Datatypes.S d))
+            | None => None
+            end) llp) x.
+Proof.
+  intro llp.
+  induction llp; intros; try easy.
+  inversion H1; subst. easy.
+  inversion H1; subst. clear H1. 
+  constructor. 
+  destruct a; try easy.
+  - right. destruct H4; try easy. destruct H1. destruct H1. destruct H1. destruct H1. destruct H2. 
+    inversion H1. subst.
+    exists (subst_expr_proc x v (Datatypes.S (length Gsl)) (Datatypes.S d)).
+    exists x0. exists x1. split; try easy. split; try easy. clear H1.
+    inversion H0; subst. clear H0.
+    specialize(H4 v (Datatypes.S d) (Some x0 :: Gsl) Gsr Gt S x1).
+    apply H4; try easy.
+    apply slideE; try easy.
+  - left. split; try easy.
+    destruct H4; try easy. destruct H1. destruct H1. destruct H1. easy.
+  - apply IHllp with (S := S); try easy.
+    inversion H0; subst. easy.
+Qed.
+
+Lemma _a24_helper : forall v d P Gsl Gsr Gt S T, 
+        typ_proc (Gsl ++ Some S :: Gsr) Gt P T -> 
+        typ_expr (Gsl ++ Gsr) (incr_freeE 0 d v) S -> 
+        typ_proc (Gsl ++ Gsr) Gt (subst_expr_proc P v (length Gsl) d) T.
+Proof.
+  intros v d P. revert v d.
+  induction P using process_ind_ref; intros; try easy.
+  - specialize(_a23_e (p_var n) n T (Gsl ++ Some S :: Gsr) Gt H (eq_refl (p_var n))); intros.
+    destruct H1. destruct H1. destruct H2.
+    simpl. apply tc_sub with (t := x); intros; try easy.
+    constructor; try easy.
+    specialize(typable_implies_wfC H); easy.
+  - specialize(_a23_f p_inact T (Gsl ++ Some S :: Gsr) Gt H (eq_refl (p_inact))); intros.
+    subst. simpl. constructor.
+  - simpl.
+    specialize(_a23_bf pt lb ex P (p_send pt lb ex P) (Gsl ++ Some S :: Gsr) Gt T H (eq_refl (p_send pt lb ex P))); intros.
+    destruct H1. destruct H1. destruct H1. destruct H2. 
+    apply tc_sub with (t := (ltt_send pt (extendLTT lb [] (Some (x, x0))))); intros; try easy.
+    constructor; try easy.
+    apply expr_subst with (S := S); try easy.
+    apply IHP with (S := S); try easy.
+    specialize(typable_implies_wfC H); try easy.
+  - specialize(_a23_a pt llp (p_recv pt llp) (Gsl ++ Some S :: Gsr) Gt T H0 (eq_refl (p_recv pt llp))); intros.
+    destruct H2. destruct H2. destruct H3. destruct H4.
+    apply tc_sub with (t := ltt_recv pt x); intros; try easy. 
+    constructor; try easy.
+    apply eq_trans with (y := length llp); try easy.
+    apply map_length; try easy. 
+    apply SList_map_a24; try easy.
+    apply _a24_helper_recv with (S := S); try easy.
+    specialize(typable_implies_wfC H0); try easy.
+  - specialize(_a23_c (p_ite e P1 P2) e P1 P2 T (Gsl ++ Some S :: Gsr) Gt H (eq_refl (p_ite e P1 P2))); intros.
+    destruct H1. destruct H1. destruct H1. destruct H2. destruct H3. destruct H4.
+    specialize(typable_implies_wfC H); intros.
+    constructor.
+    apply expr_subst with (S := S); try easy.
+    apply IHP1 with (S := S); try easy.
+    apply tc_sub with (t := x); try easy.
+    apply IHP2 with (S := S); try easy.
+    apply tc_sub with (t := x0); try easy.
+  - specialize(_a23_d (p_rec P) P T (Gsl ++ Some S :: Gsr) Gt H (eq_refl (p_rec P))); intros.
+    destruct H1. destruct H1.
+    apply tc_sub with (t := x); try easy.
+    simpl in *. constructor. apply IHP with (S := S); try easy.
+    specialize(typable_implies_wfC H); try easy. 
+Qed.
+
+Lemma _a24 : forall v Gs Gt P S T,
+        typ_proc (Some S :: Gs) Gt P T -> 
+        typ_expr Gs v S -> 
+        typ_proc Gs Gt (subst_expr_proc P v 0 0) T.
+Proof.
+  intros. 
+  specialize(_a24_helper v 0 P nil Gs Gt S T); intros. simpl in H1. apply H1; try easy.
+  specialize(trivial_incrE 0 v); intros. replace (incr_freeE 0 0 v) with v. easy.
+Qed.
+    
+
+(* 
 #[global] Declare Instance RW_scong3: Proper (scong ==> scong ==> impl) betaP.
 #[global] Declare Instance RW_scong4: Proper (scong ==> scong ==> impl) beta_multistep.
-
-Definition PAlice: process := 
+ *)
+(* Definition PAlice: process := 
   p_send "Bob" 1 (e_val (vint 50)) (p_recv "Carol" [None; None; None; Some p_inact]).
 
 Definition PBob: process :=
@@ -85,9 +325,8 @@ Definition PCarol: process :=
 
 Definition MS: session := ("Alice" <-- Some PAlice) ||| ("Bob" <-- Some PBob) ||| ("Carol" <-- Some PCarol).
 
-Definition MS': session := ("Alice" <-- Some p_inact) ||| ("Bob" <-- Some p_inact) ||| ("Carol" <-- Some p_inact).
+Definition MS': session := ("Alice" <-- Some p_inact) ||| ("Bob" <-- Some p_inact) ||| ("Carol" <-- Some p_inact). *)
 
-Eval compute in (eval_expr (e_plus (e_val (vint 100)) (e_val (vint 5)))).
 (* 
 Example redMS: beta_multistep MS MS'.
 Proof. unfold beta_multistep, MS, MS', PAlice, PBob.
