process/sessions.v
@@ -1,4 +1,4 @@
-From SST Require Export src.unscoped src.expressions process.processes process.substitution process.inversion process.typecheck type.global type.local tree.global tree.local.
+From SST Require Export src.unscoped src.expressions process.processes process.substitution process.inversion process.inversion_expr process.typecheck type.global type.local tree.global tree.local.
 Require Import List String Datatypes ZArith Relations PeanoNat.
 Open Scope list_scope.
 Require Import Setoid Morphisms Coq.Program.Basics.
@@ -22,19 +22,23 @@ Inductive ForallT (P : part -> process -> Prop) : session -> Prop :=
   | ForallT_mono : forall pt op, P pt op -> ForallT P (pt <-- op)
   | ForallT_par : forall (M1 M2 : session), ForallT P M1 -> ForallT P M2 -> ForallT P (M1 ||| M2). 
   
-
-Fixpoint InT (pt : part) (M : session) : Prop :=
+Fixpoint flattenT (M : session) : (list part) := 
   match M with 
-    | p <-- _ => p = pt 
-    | M1 |||  M2 => (InT pt M1) \/ (InT pt M2)
+    | p <-- _   => p :: nil
+    | M1 ||| M2 => flattenT M1 ++ flattenT M2
   end.
 
+Definition InT (pt : part) (M : session) : Prop :=
+  In pt (flattenT M).
+  
 Inductive typ_sess : session -> gtt -> Prop := 
   | t_sess : forall M G, (forall pt, isgPartsC pt G -> InT pt M) ->
+                         NoDup (flattenT M) ->
                          ForallT (fun u P => exists T, projectionC G u T /\ typ_proc nil nil P T) M ->
                          typ_sess M G.
 
 Lemma _a23_2 : forall M G, typ_sess M G -> (forall pt, isgPartsC pt G -> InT pt M) /\ 
+               NoDup (flattenT M) ->
                ForallT (fun u P => exists T, projectionC G u T /\ typ_proc nil nil P T) M.
 Proof.
   intros. inversion H; try easy.
@@ -44,15 +48,39 @@ Qed.
 Inductive stepE : relation expr := 
   | ec_var   : forall n, stepE (e_var n) (e_var n)
   | ec_val   : forall v, stepE (e_val v) (e_val v)
-  | ec_succ  : forall n, stepE (e_succ (e_val (vint n))) (e_val (vint (n+1))).
+  | ec_succ  : forall n, stepE (e_succ (e_val (vnat n))) (e_val (vnat (n+1)))
+  | ec_neg   : forall n, stepE (e_neg (e_val (vint n))) (e_val (vint (-n)))
+  | ec_t_f   :           stepE (e_not (e_val (vbool true))) (e_val (vbool false))
+  | ec_f_t   :           stepE (e_not (e_val (vbool false))) (e_val (vbool true))
+  | ec_gt_t  : forall m n, Z.lt n m -> stepE (e_gt (e_val (vint m)) (e_val (vint n))) (e_val (vbool true)) 
+  | ec_gt_f  : forall m n, Z.le m n -> stepE (e_gt (e_val (vint m)) (e_val (vint n))) (e_val (vbool false))
+  | ec_plus  : forall m n, stepE (e_plus (e_val (vint n)) (e_val (vint m))) (e_val (vint (n + m)))
+  | ec_detl  : forall m n v, stepE m v -> stepE (e_det m n) v
+  | ec_detr  : forall m n v, stepE n v -> stepE (e_det m n) v.
+
+Inductive multi {X : Type} (R : relation X) : relation X :=
+  | multi_refl : forall (x : X), multi R x x 
+  | multi_step : forall (x y z : X), R x y -> multi R y z -> multi R x z.
+  
+Lemma transitive_multi {X : Type} : forall (R : relation X) (x y z : X), multi R x y -> multi R y z -> multi R x z.
+Proof.
+  intros R x y z H.
+  revert z.
+  induction H; intros. easy.
+  specialize(IHmulti z0 H1).
+  specialize(@multi_step X R); intros.
+  apply H2 with (y := y). easy. easy.
+Qed.
+
+Definition stepE_multi := multi stepE.
    
 Inductive scongP : relation process := 
   | pc_inact : scongP p_inact p_inact
   | pc_var   : forall n, scongP (p_var n) (p_var n)
   | pc_mu    : forall X Y, scongP X Y -> scongP (p_rec X) (p_rec Y)
-  | pc_ite   : forall e e' X X' Y Y', stepE e e' -> scongP X X' -> scongP Y Y' -> scongP (p_ite e X Y) (p_ite e' X' Y')
+  | pc_ite   : forall e X X' Y Y', scongP X X' -> scongP Y Y' -> scongP (p_ite e X Y) (p_ite e X' Y')
   | pc_recv  : forall pt xs ys, Forall2 (fun u v => (u = None /\ v = None) \/ (exists P Q, u = Some P /\ v = Some Q /\ scongP P Q)) xs ys -> scongP (p_recv pt xs) (p_recv pt ys)
-  | pc_send  : forall pt lb e e' X X', stepE e e' -> scongP X X' -> scongP (p_send pt lb e X) (p_send pt lb e' X')
+  | pc_send  : forall pt lb e X X', scongP X X' -> scongP (p_send pt lb e X) (p_send pt lb e X')
   | pc_sub   : forall P Q, substitutionP 0 0 0 (p_rec P) P Q -> scongP (p_rec P) Q
   | pc_trans : forall P Q R, scongP P Q -> scongP Q R -> scongP P R.
 
@@ -61,9 +89,9 @@ Section scongP_ind_ref.
   Hypothesis P_inact : P p_inact p_inact.
   Hypothesis P_var   : forall n, P (p_var n) (p_var n).
   Hypothesis P_mu    : forall X Y, P X Y -> P (p_rec X) (p_rec Y).
-  Hypothesis P_ite   : forall e e' X X' Y Y', stepE e e' -> P X X' -> P Y Y' -> P (p_ite e X Y) (p_ite e' X' Y').
+  Hypothesis P_ite   : forall e X X' Y Y', P X X' -> P Y Y' -> P (p_ite e X Y) (p_ite e X' Y').
   Hypothesis P_recv  : forall pt xs ys, Forall2 (fun u v => (u = None /\ v = None) \/ (exists X Y, u = Some X /\ v = Some Y /\ P X Y)) xs ys -> P (p_recv pt xs) (p_recv pt ys).
-  Hypothesis P_send  : forall pt lb e e' X X', stepE e e' -> P X X' -> P (p_send pt lb e X) (p_send pt lb e' X').
+  Hypothesis P_send  : forall pt lb e X X', P X X' -> P (p_send pt lb e X) (p_send pt lb e X').
   Hypothesis P_sub   : forall X Y, substitutionP 0 0 0 (p_rec X) X Y -> P (p_rec X) Y.
   Hypothesis P_trans : forall X Y Z, P X Y -> P Y Z -> P X Z.
   
@@ -73,9 +101,9 @@ Section scongP_ind_ref.
       | pc_inact => P_inact
       | pc_var n => P_var n 
       | pc_mu X Y Hp => P_mu X Y (scongP_ind_ref X Y Hp)
-      | pc_ite e e' X X' Y Y' He Hx Hy => P_ite e e' X X' Y Y' He (scongP_ind_ref X X' Hx) (scongP_ind_ref Y Y' Hy)
+      | pc_ite e X X' Y Y' Hx Hy => P_ite e X X' Y Y' (scongP_ind_ref X X' Hx) (scongP_ind_ref Y Y' Hy)
       | pc_recv pt xs ys Ha => P_recv pt xs ys _
-      | pc_send pt lb e e' X X' He Hx => P_send pt lb e e' X X' He (scongP_ind_ref X X' Hx)
+      | pc_send pt lb e X X' Hx => P_send pt lb e X X' (scongP_ind_ref X X' Hx)
       | pc_sub X Y Hs => P_sub X Y Hs
       | pc_trans X Y Z Hxy Hyz => P_trans X Y Z (scongP_ind_ref X Y Hxy) (scongP_ind_ref Y Z Hyz)
     end); try easy.
@@ -96,10 +124,41 @@ Inductive scong: relation session :=
 Lemma _a22_2_helper : forall pt G, isgPartsC pt G -> projectionC G pt ltt_end -> False.
 Admitted.
 
-Lemma expr_typ_cong : forall Gs e e' S, typ_expr Gs e S -> stepE e e' -> typ_expr Gs e' S.
+Lemma expr_typ_step : forall Gs e e' S, typ_expr Gs e S -> stepE e e' -> typ_expr Gs e' S.
 Proof.
-Admitted.
+  intros. revert H. revert S. induction H0; intros; try easy.
+  - specialize(inv_expr_succ Gs (e_succ (e_val (vnat n))) S (e_val (vnat n)) H (eq_refl (e_succ (e_val (vnat n))))); intros.
+    destruct H0. destruct H1; subst.
+    apply sc_valn.
+    apply sc_sub with (s := snat). apply sc_valn. apply sni.
+  - specialize(inv_expr_neg Gs (e_neg (e_val (vint n))) S (e_val (vint n)) H (eq_refl (e_neg (e_val (vint n))))); intros.
+    destruct H0. subst. apply sc_vali.
+  - specialize(inv_expr_not Gs (e_not (e_val (vbool true))) S (e_val (vbool true)) H (eq_refl (e_not (e_val (vbool true))))); intros.
+    destruct H0. subst. apply sc_valb.
+    specialize(inv_expr_not Gs (e_not (e_val (vbool false))) S (e_val (vbool false)) H (eq_refl (e_not (e_val (vbool false))))); intros.
+    destruct H0. subst. apply sc_valb.
+  - specialize(inv_expr_gt Gs (e_gt (e_val (vint m)) (e_val (vint n))) S (e_val (vint m)) (e_val (vint n)) H0 (eq_refl (e_gt (e_val (vint m)) (e_val (vint n))))); intros.
+    destruct H1. destruct H2. subst. apply sc_valb.
+  - specialize(inv_expr_gt Gs (e_gt (e_val (vint m)) (e_val (vint n))) S (e_val (vint m)) (e_val (vint n)) H0 (eq_refl (e_gt (e_val (vint m)) (e_val (vint n))))); intros.
+    destruct H1. destruct H2. subst. apply sc_valb.
+  - specialize(inv_expr_plus Gs (e_plus (e_val (vint n)) (e_val (vint m))) S (e_val (vint n)) (e_val (vint m)) H (eq_refl (e_plus (e_val (vint n)) (e_val (vint m))))); intros.
+    destruct H0. destruct H1. subst. apply sc_vali.
+  - specialize(inv_expr_det Gs (e_det m n) S m n H (eq_refl (e_det m n))); intros.
+    destruct H1. destruct H1. destruct H2.
+    apply sc_sub with (s := x); intros; try easy. apply IHstepE; try easy.
+  - specialize(inv_expr_det Gs (e_det m n) S m n H (eq_refl (e_det m n))); intros.
+    destruct H1. destruct H1. destruct H2.
+    apply sc_sub with (s := x); intros; try easy. apply IHstepE; try easy.
+Qed.
 
+
+Lemma expr_typ_multi : forall Gs e e' S, typ_expr Gs e S -> stepE_multi e e' -> typ_expr Gs e' S.
+Proof.
+  intros. revert H. revert S. induction H0; intros; try easy.
+  apply IHmulti.
+  apply expr_typ_step with (e := x); try easy.
+Qed.
+  
 Lemma _a22_2_helperP_1 : forall xs x l' Gs Gt,
       Forall2
        (fun u v : option process =>
@@ -195,7 +254,7 @@ Proof.
       apply typable_implies_wfC with (P := (p_recv pt (a :: xs))) (Gs := Gs) (Gt := Gt); try easy.
 Qed.
 
-Lemma _a22_2_helperP : forall Gs Gt P Q T, typ_proc Gs Gt P T -> scongP P Q -> typ_proc Gs Gt Q T.
+Lemma _a22_1 : forall Gs Gt P Q T, typ_proc Gs Gt P T -> scongP P Q -> typ_proc Gs Gt Q T.
 Proof.
   intros. revert H. revert Gs Gt T.
   induction H0 using scongP_ind_ref; intros; try easy.
@@ -205,20 +264,18 @@ Proof.
     apply tc_sub with (t := x); try easy.
     apply tc_mu; try easy.
     apply typable_implies_wfC with (P := p_rec X) (Gs := Gs) (Gt := Gt); try easy.
-  - specialize(_a23_c (p_ite e X Y) e X Y T Gs Gt H0 (eq_refl (p_ite e X Y))); intros.
-    destruct H1. destruct H1. destruct H1. destruct H2. destruct H3. destruct H4.
-    apply tc_ite.
-    apply expr_typ_cong with (e := e); try easy.
+  - specialize(_a23_c (p_ite e X Y) e X Y T Gs Gt H (eq_refl (p_ite e X Y))); intros.
+    destruct H0. destruct H0. destruct H0. destruct H1. destruct H2. destruct H3.
+    apply tc_ite. easy.
     apply IHscongP; try easy. apply tc_sub with (t := x); try easy.
     apply typable_implies_wfC with (P := p_ite e X Y) (Gs := Gs) (Gt := Gt); try easy.
     apply IHscongP0; try easy. apply tc_sub with (t := x0); try easy.
     apply typable_implies_wfC with (P := p_ite e X Y) (Gs := Gs) (Gt := Gt); try easy.
   - apply _a22_2_helperP_h with (xs := xs); try easy.
-  - specialize(_a23_bf pt lb e X (p_send pt lb e X) Gs Gt T H0 (eq_refl (p_send pt lb e X))); intros.
-    destruct H1. destruct H1. destruct H1. destruct H2.
+  - specialize(_a23_bf pt lb e X (p_send pt lb e X) Gs Gt T H (eq_refl (p_send pt lb e X))); intros.
+    destruct H0. destruct H0. destruct H0. destruct H1.
     apply tc_sub with (t := (ltt_send pt (extendLTT lb nil (Some (x, x0))))); try easy.
     apply tc_send; try easy.
-    apply expr_typ_cong with (e := e); try easy.
     apply IHscongP; try easy.
     apply typable_implies_wfC with (P := p_send pt lb e X) (Gs := Gs) (Gt := Gt). easy.
   - specialize(_a23_d (p_rec X) X T Gs Gt H0 (eq_refl (p_rec X))); intros.
@@ -231,32 +288,96 @@ Proof.
   - apply IHscongP0; try easy. apply IHscongP; try easy.
 Qed.
 
+Lemma noin_mid {A} : forall (l1 l2 : list A) a a0, ~ In a0 (l1 ++ a :: l2) -> ~ In a0 (l1 ++ l2) /\ a <> a0.
+Proof.
+  induction l1; intros; try easy.
+  simpl in *.
+  specialize(Classical_Prop.not_or_and (a = a0) (In a0 l2) H); intros.
+  easy.
+  simpl in *. 
+  specialize(Classical_Prop.not_or_and (a = a1) (In a1 (l1 ++ a0 :: l2)) H); intros.
+  destruct H0.
+  specialize(IHl1 l2 a0 a1 H1). destruct IHl1.
+  split; try easy.
+  apply Classical_Prop.and_not_or. split; try easy.
+Qed.
+
+Lemma in_mid {A} : forall (l1 l2 : list A) a pt, In pt (l1 ++ a :: l2) -> (pt = a \/ In pt (l1 ++ l2)).
+Proof.
+  induction l1; intros; try easy.
+  simpl in *. destruct H. left. easy. right. easy.
+  simpl in H. destruct H. right. left. easy.
+  specialize(IHl1 l2 a0 pt H); intros. destruct IHl1. left. easy.
+  right. right. easy.
+Qed.
+
+Lemma noin_swap {A} : forall (l1 l2 : list A) a, ~ In a (l1 ++ l2) -> ~ In a (l2 ++ l1).
+Proof.
+  induction l2; intros. simpl in *.
+  specialize(app_nil_r l1); intros. replace (l1 ++ nil) with l1 in *. easy.
+  specialize(noin_mid l1 l2 a a0 H); intros. destruct H0.
+  simpl in *.
+  apply Classical_Prop.and_not_or. split; try easy.
+  apply IHl2; try easy. 
+Qed.
+
+
+Lemma nodup_swap {A} : forall (l1 l2 : list A), NoDup (l1 ++ l2) -> NoDup (l2 ++ l1).
+Proof.
+  induction l2; intros. simpl in *.
+  specialize(app_nil_r l1); intros. replace (l1 ++ nil) with l1 in *. easy.
+  specialize(NoDup_remove_1 l1 l2 a H); intros.
+  specialize(NoDup_remove_2 l1 l2 a H); intros.
+  specialize(IHl2 H0).
+  constructor; try easy.
+  apply noin_swap; try easy.
+Qed.
+
+Lemma in_swap {A} : forall (l1 l2 : list A) pt, In pt (l1 ++ l2) -> In pt (l2 ++ l1).
+Proof.
+  induction l2; intros. simpl in *.
+  specialize(app_nil_r l1); intros. replace (l1 ++ nil) with l1 in *. easy.
+  specialize(in_mid l1 l2 a pt H); intros.
+  destruct H0. left. easy. right. apply IHl2; try easy.
+Qed.
 
 Lemma _a22_2 : forall M M' G, typ_sess M G -> scong M M' -> typ_sess M' G.
 Proof.
   intros. revert H. revert G. induction H0; intros; try easy.
-  - inversion H0. subst. inversion H2. subst. clear H2.
-    inversion H5. subst. clear H5. destruct H3. destruct H2.
-    constructor; try easy. constructor; try easy. constructor; try easy. 
+  - inversion H0. subst. inversion H3. subst. clear H3.
+    inversion H6. subst. clear H6. destruct H4. destruct H3.
+    constructor; try easy. constructor. constructor; try easy.
     exists x. split; try easy.
-    apply _a22_2_helperP with (P := P); try easy.
-  - inversion H. subst. inversion H1. subst. clear H1. 
-    constructor; try easy.
-    intros. specialize(H0 pt H1).
+    apply _a22_1 with (P := P); try easy.
+    easy.
+  - inversion H. subst. inversion H2. subst. clear H2.
+    constructor; try easy. inversion H5. subst. destruct H3. destruct H2. clear H5.
+    intros. specialize(H0 pt H4).
     simpl in H0. destruct H0; try easy. subst. 
-    inversion H4. subst. destruct H2. destruct H0.
-    specialize(_a23_f p_inact x nil nil H2 (eq_refl p_inact)); intros. subst. clear H4 H5 H2.
-    specialize(_a22_2_helper pt G H1 H0); intros. easy.
+    specialize(_a23_f p_inact x nil nil H3 (eq_refl p_inact)); intros. subst. 
+    specialize(_a22_2_helper pt G H4 H2); intros. easy.
+  - simpl in H1. inversion H1. subst. easy.
   - inversion H; subst. inversion H1; subst. constructor.
-    intros. specialize (H0 pt H2); intros. simpl. 
-    destruct H0; try easy. right. easy. left. easy.
+    intros. specialize (H0 pt H3); intros. simpl.
+    apply in_swap; try easy. 
+    apply nodup_swap; try easy.
+    inversion H2. subst. constructor; try easy.
     constructor; try easy.
-  - inversion H; subst. inversion H1; subst. inversion H4; subst. clear H1 H4.
+    intros. specialize(H0 pt H6). 
+    simpl in *.
+    apply in_swap; try easy.
+    apply nodup_swap; try easy.
+  - inversion H2. subst. constructor; try easy.
+  - inversion H; subst. inversion H2; subst. inversion H5; subst. 
     constructor. 
-    - intros. specialize(H0 pt H1). simpl in *. 
-      destruct H0. destruct H0. left. easy. 
-      right. left. easy.
-      right. right. easy.
+    - intros. specialize(H0 pt H3). unfold InT in *. simpl in *.
+    specialize(app_assoc (flattenT M) (flattenT M') (flattenT M'')); intros.
+    replace (flattenT M ++ flattenT M' ++ flattenT M'') with ((flattenT M ++ flattenT M') ++ flattenT M'') in *.
+    easy.
+    simpl in *.
+    specialize(app_assoc (flattenT M) (flattenT M') (flattenT M'')); intros.
+    replace (flattenT M ++ flattenT M' ++ flattenT M'') with ((flattenT M ++ flattenT M') ++ flattenT M'') in *.
+    easy.
     constructor; try easy. constructor; try easy.
 Qed.
 
