process/subject_reduction.v
@@ -1,6 +1,7 @@
 From SST Require Export src.unscoped src.expressions process.processes process.typecheck type.global type.local tree.global tree.local process.beta process.sessions process.inversion.
 Require Import List String Datatypes ZArith Relations PeanoNat.
 Open Scope list_scope.
+From Paco Require Import paco pacotac.
 Require Import Setoid Morphisms Coq.Program.Basics.
 Require Import Coq.Init.Datatypes.
 
@@ -9,52 +10,384 @@ Inductive multiC : relation gtt :=
   | multiC_step : forall G1 G2 G3 p q n, gttstepC G1 G2 p q n -> multiC G2 G3 -> multiC G1 G3.
 
 
+Lemma projection_cont_p : forall G x6 p q l x,
+    gttstepC G x6 q p l -> projectionC G p (ltt_recv q x) -> exists T, projectionC x6 p T.
+Proof.
+  intros. revert H0. revert x.
+  
+  
+  induction H using gttstepC_ind_ref.
+  - intros.
+    pinversion H1; try easy.
+    - assert (isgPartsC q (gtt_send p q xs)). { pfold. constructor. }
+      specialize(H2 H6). easy. 
+    subst. 
+    admit.
+  admit.
+  - intros.
+    
+  - intros. subst.
+    - admit.
+  - admit.
+Admitted.
+
+Lemma projection_cont_q : forall G x6 p q l x0,
+    gttstepC G x6 q p l -> projectionC G q (ltt_send p x0) -> exists T, projectionC x6 q T.
+Admitted.
+
+Lemma projection_cont_r : forall G x6 q p0 l s x,
+    projectionC G s x ->
+    gttstepC G x6 q p0 l -> 
+    q <> s ->
+    p0 <> s ->
+    exists T, projectionC x6 s T.
+Admitted.
+
+Lemma projection_wfc_p : forall G l p q x4 x8 x9, 
+        wfC (ltt_recv q x4) ->
+        projectionC G p (ltt_recv q x4) ->
+        gttstepC G x8 q p l ->
+        projectionC x8 p x9 ->
+        wfC x9.
+Admitted.
+
+Lemma projection_wfc_q : forall G l p q x x8 x9,
+        wfC (ltt_send p x) ->
+        projectionC G q (ltt_send p x) ->
+        gttstepC G x8 q p l ->
+        projectionC x8 q x9 ->
+        wfC x9.
+Admitted.
+
+Lemma projection_wfc_r : forall G l p0 q s x x0 x6,
+        wfC x ->
+        q <> s ->
+        p0 <> s ->
+        projectionC G s x ->
+        gttstepC G x6 q p0 l ->
+        projectionC x6 s x0 ->
+        wfC x0.
+Admitted.
+
+Lemma _3_19_h : forall p q l G L1 L2 S T xs y,
+  projectionC G p (ltt_send q L1) -> 
+  subtypeC (ltt_send q (extendLTT l nil (Datatypes.Some(S,T)))) (ltt_send q L1) ->
+  projectionC G q (ltt_recv p L2) -> 
+  onth l xs = Some y ->
+  subtypeC (ltt_recv p xs) (ltt_recv p L2) -> 
+  exists G', gttstepC G G' p q l.
+Proof.
+  intros. 
+  pinversion H0. subst.
+  pinversion H1; subst; try easy.
+  - admit.
+  - admit.
+Admitted.
+
+Lemma _3_19_1 : forall p q l G G' L1 L2 S T,
+  projectionC G p (ltt_send q L1) ->
+  subtypeC (ltt_send q (extendLTT l nil (Datatypes.Some (S,T)))) (ltt_send q L1) ->
+  gttstepC G G' p q l ->
+  projectionC G' p L2 ->
+  subtypeC T L2.
+Admitted.
+
+Lemma _3_19_2 : forall p q l G G' L1 L2 S T xs,
+  projectionC G q (ltt_recv p L1) -> 
+  subtypeC (ltt_recv p xs) (ltt_recv p L1) ->
+  onth l xs = Some (S, T) ->
+  gttstepC G G' p q l -> 
+  projectionC G' q L2 ->
+  subtypeC T L2.
+Admitted.
+
+Lemma _3_19_3 : forall p q r l G G' L1 L2,
+  r <> p -> r <> q ->
+  projectionC G r L1 ->
+  gttstepC G G' p q l -> 
+  projectionC G' r L2 -> 
+  subtypeC L1 L2.
+Proof.
+  
+Admitted.
+
+Lemma onth_follow : forall l xs y x1,
+  onth l xs = Some y ->
+  Forall2
+       (fun (u : option process) (v : option (sort * ltt)) =>
+        u = None /\ v = None \/
+        (exists (p : process) (s : sort) (t : ltt),
+           u = Some p /\ v = Some (s, t) /\ typ_proc (Some s :: nil) nil p t))
+       xs x1 ->
+  exists s t, onth l x1 = Some (s, t).
+Proof.
+  induction l; intros; try easy.
+  destruct xs; subst. easy.
+  inversion H0; subst. clear H0. simpl in *. subst. 
+  - destruct H3. easy. destruct H. destruct H. destruct H. destruct H. destruct H0. inversion H. inversion H0. subst.
+    exists x0. exists x1. easy.
+  - destruct xs. easy.
+    destruct x1; try easy.
+    simpl in *.
+    inversion H0. subst. clear H0. apply IHl with (xs := xs) (y := y); try easy.
+Qed.
+
+Lemma _3_21_1_helper : forall l x1 xs x4 x5 y,
+    onth l x1 = Some (x4, x5) ->
+    onth l xs = Some y ->
+    Forall2
+       (fun (u : option process) (v : option (sort * ltt)) =>
+        u = None /\ v = None \/
+        (exists (p : process) (s : sort) (t : ltt),
+           u = Some p /\ v = Some (s, t) /\ typ_proc (Some s :: nil) nil p t))
+       xs x1 ->
+    typ_proc (Some x4 :: nil) nil y x5.
+Proof.
+  induction l; intros; try easy.
+  - destruct x1. try easy. destruct xs. try easy.
+    simpl in *. subst.
+    inversion H1. subst. destruct H3. destruct H. easy.
+    destruct H. destruct H. destruct H. destruct H. destruct H0. inversion H. inversion H0. subst. easy.
+  - destruct x1; try easy. destruct xs; try easy.
+    simpl in *. apply IHl with (x1 := x1) (xs := xs); try easy.
+    inversion H1; try easy.
+Qed.
+
+Lemma noin_cat_and {A} : forall pt (l1 l2 : list A), ~ In pt (l1 ++ l2) -> ~ (In pt l1 \/ In pt l2).
+Proof.
+  induction l1; intros; try easy.
+  simpl in *. apply Classical_Prop.and_not_or. split; try easy.
+  simpl in *. specialize(Classical_Prop.not_or_and (a = pt) (In pt (l1 ++ l2)) H); intros.
+  destruct H0. 
+  apply Classical_Prop.and_not_or.
+  specialize(IHl1 l2 H1).
+  specialize(Classical_Prop.not_or_and (In pt l1) (In pt l2) IHl1); intros. destruct H2.
+  split; try easy. apply Classical_Prop.and_not_or. split; try easy.
+Qed.
+
+Lemma _3_21_3_helper : forall M p q x6 G l,
+    ForallT
+       (fun (u : string) (P : process) =>
+        exists T : ltt, projectionC G u T /\ typ_proc nil nil P T) M ->
+    gttstepC G x6 q p l ->
+    ~ InT q M ->
+    ~ InT p M ->
+    ForallT
+      (fun (u : string) (P : process) =>
+       exists T : ltt, projectionC x6 u T /\ typ_proc nil nil P T) M.
+Proof.
+  intro M. induction M; intros; try easy.
+  - constructor; try easy.
+    inversion H. subst. destruct H4. destruct H3.
+    specialize(projection_cont_r G x6 q p0 l s x H3 H0); intros.
+    assert (q <> s). { 
+      unfold InT in H1. simpl in H1. 
+      specialize(Classical_Prop.not_or_and (s = q) False H1); intros. destruct H6.
+      easy.
+    }
+    assert (p0 <> s). {
+      unfold InT in H2. simpl in H2.
+      specialize(Classical_Prop.not_or_and (s = p0) False H2); intros. destruct H7.
+      easy.
+    }
+    specialize(H5 H6 H7). destruct H5.
+    exists x0.
+    split; try easy.
+    apply tc_sub with (t := x); try easy.
+    specialize(_3_19_3 q p0 s l G x6 x x0); intros.
+    apply H8; try easy.
+    assert (wfC x0). { 
+        specialize(projection_wfc_r G l p0 q s x x0 x6); intros.
+        apply H8; try easy.
+        specialize(typable_implies_wfC H4). easy.
+    } easy. 
+  - inversion H. subst. simpl in *.
+    unfold InT in *. simpl in *.
+    specialize(noin_cat_and q (flattenT M1) (flattenT M2) H1); intros.
+    specialize(noin_cat_and p (flattenT M1) (flattenT M2) H2); intros.
+    specialize(Classical_Prop.not_or_and (InT q M1) (InT q M2) H3); intros. destruct H7. 
+    specialize(Classical_Prop.not_or_and (InT p M1) (InT p M2) H4); intros. destruct H9.
+    constructor. apply IHM1 with (p := p) (q := q) (G := G) (l := l); try easy.
+    apply IHM2 with (p := p) (q := q) (G := G) (l := l); try easy.
+Qed.
+
+Lemma part_step : forall pt G x6 q p l,
+    isgPartsC pt x6 ->
+    gttstepC G x6 q p l ->
+    isgPartsC pt G.
+Proof.
+Admitted.
+
+Lemma _3_21_ssort_helper : forall l x x2 x3,
+      Forall2
+        (fun u v : option (sort * ltt) =>
+         u = None \/
+         (exists (s s' : sort) (t t' : ltt),
+            u = Some (s, t) /\ v = Some (s', t') /\ subsort s s' /\ subtypeC t t'))
+        (extendLTT l nil (Some (x2, x3))) x ->
+      exists y z, onth l x = (Some (y, z)) /\ subsort x2 y.
+Proof.
+  induction l; intros; try easy.
+  - destruct x; try easy. simpl in *.
+    destruct o. destruct p. exists s. exists l. split; try easy.
+    inversion H. subst. destruct H3; try easy. 
+    destruct H0. destruct H0. destruct H0. destruct H0. destruct H0. destruct H1. destruct H2.
+    inversion H0. inversion H1. subst. easy.
+    inversion H. subst. destruct H3; try easy.
+    destruct H0. destruct H0. destruct H0. destruct H0. destruct H0. destruct H1. easy.
+  - destruct x; try easy. simpl in *.
+    inversion H. subst. apply IHl with (x3 := x3); try easy.
+Qed.
+
+Lemma _3_21_ssort_helper2 : forall G p q x x8,
+      projectionC G p (ltt_recv q x8) ->
+      projectionC G q (ltt_send p x) ->
+      List.Forall2 (fun u v => (u = None /\ v = None) \/ (exists s t t', u = Some(s,t) /\ v = Some(s,t'))) x8 x.
+Proof.
+  induction x; intros; try easy.
+  destruct x8; try easy.
+Admitted.
+
+Lemma _3_21_ssort_helper3 : forall l x x8 x0 x9,
+      Forall2
+        (fun u v : option (sort * ltt) =>
+         u = None /\ v = None \/ (exists (s : sort) (t t' : ltt), u = Some (s, t) /\ v = Some (s, t')))
+        x8 x ->
+      onth l x = Some (x0, x9) ->
+      exists x10, onth l x8 = Some(x0, x10).
+Proof.
+  induction l; intros; try easy.
+  destruct x; try easy. destruct x8; try easy. simpl in *.
+  inversion H. subst. destruct H4; try easy.
+  destruct H0. destruct H0. destruct H0. destruct H0. inversion H1. subst. exists x2. easy.
+  destruct x; try easy. destruct x8; try easy. inversion H. subst. simpl in *.
+  apply IHl with (x := x) (x9 := x9); try easy.
+Qed.
+
+Lemma _3_21_ssort_helper4 : forall l x1 x4 x5 x8 x0 x10,
+      onth l x1 = Some (x4, x5) ->
+      onth l x8 = Some (x0, x10) ->
+      Forall2
+        (fun u v : option (sort * ltt) =>
+         v = None \/
+         (exists (s s' : sort) (t t' : ltt),
+            u = Some (s, t) /\ v = Some (s', t') /\ subsort s' s /\ subtypeC t t')) x1 x8 ->
+      subsort x0 x4.
+Proof.
+  induction l; intros; try easy.
+  - destruct x1; try easy. destruct x8; try easy. simpl in *. 
+    inversion H1. subst. destruct H5; try easy.
+    destruct H. destruct H. destruct H. destruct H. destruct H. destruct H0. destruct H2. 
+    inversion H. inversion H0. subst. easy.
+  - destruct x1; try easy. destruct x8; try easy. simpl in *.
+    inversion H1. subst.
+    specialize(IHl x1 x4 x5 x8 x0 x10 H H0 H7).
+    easy.
+Qed.
 
 Theorem _3_21 : forall M M' G, typ_sess M G -> betaP M M' -> exists G', typ_sess M' G' /\ multiC G G'.
 Proof.
   intros. revert H. revert G.
   induction H0; intros; try easy.
   (* R-COMM *)
-  inversion H. subst. inversion H1. subst. clear H1. inversion H4. subst. clear H4.
-  inversion H3. subst. clear H3. inversion H6. subst. clear H6.
-  - destruct H2. destruct H1. destruct H1. destruct H2. inversion H2. subst. clear H2.
-    destruct H3. destruct H2. destruct H2. destruct H3. inversion H3. subst. clear H3.
-  - specialize(_a23_a q xs (p_recv q xs) nil nil x H4 (eq_refl (p_recv q xs))); intros.
-    destruct H3. destruct H3. destruct H7. destruct H8. 
-  - specialize(_a23_bf p l e Q (p_send p l e Q) nil nil x0 H6 (eq_refl (p_send p l e Q))); intros.
-    destruct H10. destruct H10. destruct H10. destruct H11. 
-  - 
+  inversion H1. subst. clear H1. inversion H3. subst. clear H3.
+  inversion H4. subst. clear H4. inversion H5. subst. clear H5.
+  - inversion H4. subst. destruct H3. destruct H1. inversion H9. subst. destruct H10. destruct H5. 
+  - specialize(_a23_a q xs (p_recv q xs) nil nil x H3 (eq_refl (p_recv q xs))); intros.
+    destruct H11. destruct H11. destruct H12. destruct H13. 
+  - specialize(_a23_bf p l e Q (p_send p l e Q) nil nil x0 H10 (eq_refl (p_send p l e Q))); intros.
+    destruct H15. destruct H15. destruct H15. destruct H16.
+  - specialize(subtype_recv x q x1 H12); intros.
+    destruct H18. subst.
+    specialize(subtype_recv_inv q x1 x4 H12); intros.
+    specialize(subtype_send x0 p (extendLTT l nil (Some (x2, x3))) H17); intros.
+    destruct H19. subst.
+    specialize(subtype_send_inv p (extendLTT l nil (Some (x2, x3))) x H17); intros.
+    specialize(_3_21_ssort_helper l x x2 x3 H19); intros.
+    destruct H20. destruct H20. destruct H20.
+  specialize(onth_follow l xs y x1 H H13); intros. destruct H22. destruct H22.
+  specialize(_3_19_h q p l G x x4 x2 x3 x1 (x6, x7) H5 H17 H1 H22 H12); intros. 
+  destruct H23. exists x8.
+  split.
+  constructor. 
+  - intros. unfold InT. simpl.
+    unfold InT in H2. simpl in H2. 
+    apply H2; try easy.
+    apply part_step with (x6 := x8) (q := q) (p := p) (l := l); try easy.
+  - simpl in *. constructor. simpl.
+    apply Classical_Prop.and_not_or.
+    specialize(Classical_Prop.not_or_and (q = p) (In p (flattenT M)) H6); intros. destruct H20.
+    split; try easy. easy.
+  constructor. constructor. constructor.
+  - specialize(_3_19_2 q p l G x8); intros.
+    specialize(projection_cont_p G x8 p q l x4 H23 H1); intros.
+    destruct H25. 
+    specialize(H24 x4 x9 x6 x7 x1 H1 H12 H22 H23 H25). 
+    exists x9. split; try easy.
+    apply _a24 with (S := x6); try easy.
+    apply tc_sub with (t := x7); intros; try easy.
+    apply _3_21_1_helper with (l := l) (x1 := x1) (xs := xs); try easy.
+    assert(wfC x9). { 
+        specialize(projection_wfc_p G l p q x4 x8 x9); intros.
+        apply H26; try easy.
+        specialize(typable_implies_wfC H3). easy.
+    } 
+    easy.
+    assert(subsort x2 x6). { 
+      apply sstrans with (s2 := x0); try easy.
+      specialize(_3_21_ssort_helper2 G p q x x4 H1 H5); intros.
+      specialize(_3_21_ssort_helper3 l x x4 x0 x5 H26 H20); intros.
+      destruct H27.
+      specialize(_3_21_ssort_helper4 l x1 x6 x7 x4 x0 x10); intros.
+      apply H28; try easy.
+    }
+    apply sc_sub with (s := x2); try easy.
+    apply expr_typ_multi with (e := e); try easy.
+  - specialize(_3_19_1 q p l G x8 x); intros.
+    specialize(projection_cont_q G x8 p q l x H23 H5); intros.
+    destruct H25.
+    specialize(H24 x9 x2 x3 H5 H17 H23 H25).
+    constructor. exists x9. split; try easy.
+    apply tc_sub with (t := x3); try easy.
+    assert(wfC x9). { 
+          specialize(projection_wfc_q G l p q x x8 x9); intros.
+          apply H26; try easy.
+          specialize(typable_implies_wfC H10). easy.
+    } 
+    easy.
+  - apply _3_21_3_helper with (p := p) (q := q) (G := G) (l := l); try easy.
+    inversion H7. subst. easy.
+    simpl in H6. specialize(Classical_Prop.not_or_and (q = p) (In p (flattenT M)) H6); intros. 
+    destruct H20; try easy.
   
-  admit.
+  apply multiC_step with (G2 := x8) (p := q) (q := p) (n := l). easy. apply multiC_refl.
   
   (* T-COND *)
-  inversion H. subst. 
-  inversion H1. subst. clear H1.
-  inversion H4. subst. clear H4. destruct H2. destruct H1. destruct H1. destruct H2.
-  inversion H2. subst. clear H2.
+  inversion H0. subst. 
+  inversion H3. subst. clear H3.
+  inversion H6. subst. clear H6. destruct H4. destruct H3. 
+  specialize(_a23_c (p_ite e P Q) e P Q x nil nil H4 (eq_refl (p_ite e P Q))); intros.
+  destruct H5. destruct H5. destruct H5. destruct H6. destruct H8. destruct H9. 
   exists G. split.
   apply t_sess; try easy. apply ForallT_par; try easy.
-  apply ForallT_mono; try easy. exists x. exists P.
-  split; try easy. split; try easy.
-  specialize(_a23_c (p_ite (e_val (vbool true)) P Q) (e_val (vbool true)) P Q x nil nil H3 (eq_refl (p_ite (e_val (vbool true)) P Q))); intros.
-  destruct H2. destruct H2. destruct H2. destruct H4. destruct H6.
+  apply ForallT_mono; try easy. exists x.
+  split; try easy.
   apply tc_sub with (t := x0); try easy.
-  specialize(typable_implies_wfC H3); try easy.
+  specialize(typable_implies_wfC H4); try easy.
   apply multiC_refl.
   
   (* F-COND *)
-  inversion H. subst. 
-  inversion H1. subst. clear H1.
-  inversion H4. subst. clear H4. destruct H2. destruct H1. destruct H1. destruct H2.
-  inversion H2. subst. clear H2.
+  inversion H0. subst. 
+  inversion H3. subst. clear H3.
+  inversion H6. subst. clear H6. destruct H4. destruct H3. 
+  specialize(_a23_c (p_ite e P Q) e P Q x nil nil H4 (eq_refl (p_ite e P Q))); intros.
+  destruct H5. destruct H5. destruct H5. destruct H6. destruct H8. destruct H9. 
   exists G. split.
   apply t_sess; try easy. apply ForallT_par; try easy.
-  apply ForallT_mono; try easy. exists x. exists Q.
-  split; try easy. split; try easy.
-  specialize(_a23_c (p_ite (e_val (vbool false)) P Q) (e_val (vbool false)) P Q x nil nil H3 (eq_refl (p_ite (e_val (vbool false)) P Q))); intros.
-  destruct H2. destruct H2. destruct H2. destruct H4. destruct H6. destruct H7.
+  apply ForallT_mono; try easy. exists x.
+  split; try easy.
   apply tc_sub with (t := x1); try easy.
-  specialize(typable_implies_wfC H3); try easy.
+  specialize(typable_implies_wfC H4); try easy.
   apply multiC_refl.
   
   (* R-STRUCT *)
@@ -63,4 +396,4 @@ Proof.
   destruct H4. split; try easy.
   specialize(_a22_2 M2' M2 x H4 H0); intros. easy.
   
-Admitted.
+Qed.
