tree/inversion.v
@@ -1,6 +1,12 @@
 From SST Require Export tree.global tree.local.
-Require Import List String.
-Open Scope string_scope.
+From mathcomp Require Import all_ssreflect.
+From SST Require Import src.coseq src.expressions.
+From Paco Require Import paco pacotac.
+Require Import String List ZArith.
+Local Open Scope string_scope.
+Import ListNotations.
+Require Import Coq.Logic.Classical_Pred_Type Coq.Logic.ClassicalFacts Coq.Logic.Classical_Prop.
+
 
 
 
