tree/paco_test.v
@@ -1,0 +1,32 @@
+Require Import Setoid Program.
+From Paco Require Import paco.
+Require Import List.
+Import ListNotations Datatypes.
+
+CoInductive box : Type :=   
+  | box_end : box
+  | cons : list (option box) -> box.
+
+Fixpoint wrel (R : box -> box -> Prop) (xs ys : list (option box)) : Prop := 
+  match (xs, ys) with 
+    | (Some x :: l1, Some y :: l2) => R x y /\ wrel R l1 l2
+    | (None :: l1, None :: l2)     => wrel R l1 l2
+    | (_, _) => False
+  end.
+
+Inductive rel (R : box -> box -> Prop) : box -> box -> Prop := 
+  | rel_end : rel R box_end box_end
+  | rel_con : forall xs ys, 
+              wrel R xs ys -> rel R (cons xs) (cons ys).
+
+Definition relC l1 l2 := paco2 rel bot2 l1 l2.
+
+Lemma relC_inv : forall x xs y ys, relC (cons (Some x :: xs)) (cons (Some y :: ys)) -> relC x y.
+Proof.
+  pcofix CIH.
+  intros.
+  pinversion H0. subst. simpl in H2. destruct H2.
+Admitted.
+
+
+
